src/SepLogic/Pred.v
@@ -1,3 +1,4 @@
 Require Export
         SepLogic.Pred.Def
-        SepLogic.Pred.Ptsto.
+        SepLogic.Pred.Ptsto
+        SepLogic.Pred.Impl.
