src/SepLogic/Pred/Impl.v
@@ -1,0 +1,8 @@
+Require Import SepLogic.Pred.Def.
+
+Theorem lift1_left : forall (P: Prop) `(q: pred A V),
+    (P -> [| True |] ===> q) ->
+    [| P |] ===> q.
+Proof.
+  unfold pimpl; simpl; intuition.
+Qed.
